Utility.v
@@ -1,0 +1,63 @@
+Require Import Lists.List Strings.String ZArith.
+
+From QuickChick Require Import QuickChick.
+Open Scope qc_scope.
+Set Warnings "-extraction-opaque-accessed,-extraction".
+
+Import ListNotations.
+Import MonadNotation.
+
+Fixpoint remove {A : Type} (n : nat) (xs : list A) :=
+  match n with
+  | O => xs
+  | S n' =>
+      match xs with
+      | [] => []
+      | x::xs' => x::(remove n' xs')
+      end
+  end.
+
+Definition rand_select_remove {A : Type} (def : A) (xs : list A) : G (A * list A) :=
+  match xs with
+  | [] => ret (def, xs)
+  | _ => (choose (0, List.length xs - 1))
+          >>= (fun n => let elem := List.nth n xs def in
+                     ret (elem, remove n xs))
+  end.
+
+Definition rand_select {A : Type} (def : A) (xs : list A) : G A :=
+  let fix rand_select' (n : nat) (xs : list A) : G A :=
+    match xs with
+    | [] => ret def
+    | x::xs' => if n =? 0 then ret x else rand_select' (n - 1) xs'
+    end in
+  (choose (0, List.length xs))
+    >>= (fun n => rand_select' n xs).
+
+Fixpoint rand_select_n {A : Type} (n : nat) (def : A) (xs : list A) : G (list A) :=
+  match n with
+  | O => ret []
+  | S n' =>
+      (rand_select_remove def xs)
+        >>= (fun '(r, xs') =>
+               (rand_select_n n' def xs')
+                 >>= (fun rs =>
+                        ret (r :: rs)))
+  end.
+
+Definition mapM@{d c +}
+           {m : Type@{d} -> Type@{c}}
+           {M : Monad m}
+           {a b} : (a -> m b) -> list a -> m (list b) :=
+  fun f =>
+    let k a r := (f a)
+                   >>= (fun x => r
+                                >>= (fun xs => ret (x::xs))) in
+    fun xs =>
+      List.fold_right k (ret []) xs.
+
+Definition sequenceM@{d c}
+           {m : Type@{d} -> Type@{c}}
+           {M : Monad m}
+           {a} : list (m a) -> m (list a) :=
+  mapM (fun x => x).
